@prefix : <http://www.sirma.com/ontologies/2014/07/tcrmConfiguration#> .
@prefix dc: <http://purl.org/dc/elements/1.1/> .
@prefix emf: <http://ittruse.ittbg.com/ontology/enterpriseManagementFramework#> .
@prefix owl: <http://www.w3.org/2002/07/owl#> .
@prefix rdf: <http://www.w3.org/1999/02/22-rdf-syntax-ns#> .
@prefix xml: <http://www.w3.org/XML/1998/namespace> .
@prefix xsd: <http://www.w3.org/2001/XMLSchema#> .
@prefix ptop: <http://www.ontotext.com/proton/protontop#> .
@prefix rdfs: <http://www.w3.org/2000/01/rdf-schema#> .
@prefix skos: <http://www.w3.org/2004/02/skos/core#> .
@prefix tcrm: <http://www.sirma.com/ontologies/2014/07/tcrmConfiguration#> .
@prefix dcterms: <http://purl.org/dc/terms/> .
@base <http://www.sirma.com/ontologies/2014/07/tcrmConfiguration> .

<http://www.sirma.com/ontologies/2014/07/tcrmConfiguration> rdf:type owl:Ontology ;
                                                            
                                                            rdfs:label "Trade and Customer Relationship Management Model"@en ;
                                                            
                                                            dc:creator "Lidiya Dimitrova" ;
                                                            
                                                            dc:subject "Trade and Customer Relationship Management Model"@en ;
                                                            
                                                            owl:versionInfo "v 1.0" ;
                                                            
                                                            skos:definition """Trade and Customer Relationship Management
TCRM Ontology"""@en ;
                                                            
                                                            owl:imports <http://ittruse.ittbg.com/ontology/enterpriseManagementFramework> .


#################################################################
#
#    Object Properties
#
#################################################################


###  http://www.sirma.com/ontologies/2014/07/tcrmConfiguration#isOrderBy

:isOrderBy rdf:type owl:ObjectProperty ;
           
           rdfs:label "is order by"@en ;
           
           dc:creator "Lidiya Dimitrova" ;
           
           skos:definition "Relationship between Product and Customer. The product is ordered by customer."@en ;
           
           rdfs:range emf:Customer ;
           
           rdfs:domain :Product ;
           
           owl:inverseOf :sendsAnOrderFor .



###  http://www.sirma.com/ontologies/2014/07/tcrmConfiguration#isProducedBy

:isProducedBy rdf:type owl:ObjectProperty ;
              
              rdfs:label "produced by"@en ;
              
              dc:creator "Lidiya Dimitrova" ;
              
              skos:definition "Relationship between Product and Factory. The product is produced by factory."@en ;
              
              rdfs:range :Factory ;
              
              rdfs:domain :Product ;
              
              owl:inverseOf :produces .



###  http://www.sirma.com/ontologies/2014/07/tcrmConfiguration#produces

:produces rdf:type owl:ObjectProperty ;
          
          rdfs:label "produces"@en ;
          
          dc:creator "Lidiya DImitrova" ;
          
          skos:definition "Relationship between Factory and Product. The product is produced by a factory."@en ;
          
          rdfs:domain :Factory ;
          
          rdfs:range :Product .



###  http://www.sirma.com/ontologies/2014/07/tcrmConfiguration#sendsAnOrderFor

:sendsAnOrderFor rdf:type owl:ObjectProperty ;
                 
                 rdfs:label "sends an order for"@en ;
                 
                 dc:creator "Lidiya DImitrova" ;
                 
                 skos:definition "Relationship between Product and Customer. The product is ordered by customer."@en ;
                 
                 rdfs:domain emf:Customer ;
                 
                 rdfs:range :Product .





#################################################################
#
#    Data properties
#
#################################################################


###  http://www.sirma.com/ontologies/2014/07/tcrmConfiguration#address

:address rdf:type owl:DatatypeProperty ;
         
         rdfs:label "Address"@en ;
         
         skos:definition "An address is a collection of information, presented in a mostly fixed format, used for describing the location of a building, apartment, or other structure or a plot of land, generally using political boundaries and street names as references, along with other identifiers such as house or apartment numbers. "@en ;
         
         dc:creator "Lidiya Dimitrova"@en .



###  http://www.sirma.com/ontologies/2014/07/tcrmConfiguration#articleNumber

:articleNumber rdf:type owl:DatatypeProperty ;
               
               rdfs:label "Article Number"@en ;
               
               dc:creator "Lidiya Dimitrova" ;
               
               skos:definition "Unique product identifier"@en ;
               
               rdfs:domain :Product .



###  http://www.sirma.com/ontologies/2014/07/tcrmConfiguration#country

:country rdf:type owl:DatatypeProperty ;
         
         rdfs:label "Country"@en ;
         
         dc:creator "Lidiya Dimitrova" ;
         
         skos:definition "A country is a region identified as a distinct entity in political geography."@en .



###  http://www.sirma.com/ontologies/2014/07/tcrmConfiguration#id

:id rdf:type owl:DatatypeProperty ;
    
    rdfs:label "Identifier/VAT number"@en ;
    
    skos:definition "Company identifier/VAT number"@en ;
    
    dc:creator "Lidiya Dimitrova" .





#################################################################
#
#    Classes
#
#################################################################


###  http://ittruse.ittbg.com/ontology/enterpriseManagementFramework#Customer

emf:Customer emf:isPartOfObjectLibrary "true"^^xsd:boolean .



###  http://www.sirma.com/ontologies/2014/07/tcrmConfiguration#Factory

:Factory rdf:type owl:Class ;
         
         rdfs:label "Factory"@en ;
         
         rdfs:subClassOf ptop:Agent ,
                         :TCRMDomainObject ;
         
         emf:isSearchable "true"^^xsd:boolean ;
         
         emf:isPartOfObjectLibrary "true"^^xsd:boolean ;
         
         dc:creator "Lidiya Dimitrova" ;
         
         skos:definition "Factory is the seat of some kind of production"@en .



###  http://www.sirma.com/ontologies/2014/07/tcrmConfiguration#Product

:Product rdf:type owl:Class ;
         
         rdfs:label "Product"@en ;
         
         rdfs:subClassOf :TCRMDomainObject ;
         
         emf:isPartOfObjectLibrary "true"^^xsd:boolean ;
         
         emf:isSearchable "true"^^xsd:boolean ;
         
         skos:definition "A product is anything that can be offered to a market that might satisfy a want or need."@en ;
         
         dc:creator "Lidiya Dimitrova" .



###  http://www.sirma.com/ontologies/2014/07/tcrmConfiguration#TCRMDomainObject

:TCRMDomainObject rdf:type owl:Class ;
                  
                  rdfs:label "TCRM Domain Object"@en ;
                  
                  rdfs:subClassOf emf:DomainObject ;
                  
                  dc:creator "Lidiya Dimitrova" ;
                  
                  skos:definition "Main Class for the TCRM Domain model"@en .




###  Generated by the OWL API (version 3.4.2) http://owlapi.sourceforge.net

